\documentclass[letterpage]{article}

\input{../common_preambles}

\begin{document}
\begin{align}
  g(x)& =e^{-a(x-b)^2}\\
  \frac{dg(x)}{dx}& = -2a(x-b)g(x)
\end{align}
Fourier transform pair is defined to be,
\begin{equation}
  G(w) = F\{g(x)\} = \int_{-\infty}^\infty g(x)e^{iwx}dx
\end{equation}
Then,
\begin{equation}
  \frac{dG(w)}{dw} = \int_{-\infty}^\infty ixg(x)e^{iwx}dx = F\{ixg(x)\}
\end{equation}
Taking the Fourier transform of both sides of (1), we get
\begin{align}
  -iwG(w) &= -2a \left(\frac{1}{i} \frac{dG(w)}{dw} - bG(w)\right)\\
  \left(ib-\frac{w}{2a}\right) G(w) &= \frac{dG(w)}{dw} \Rightarrow
    \frac{1}{G(w)} \frac{dG(w)}{dw} = ib-\frac{w}{2a}\\
  \int_0^w \frac{1}{G(w)'} \frac{dG(w)'}{dw'} dw' &= 
    \arrowvert\ln G(w')\arrowvert_0^w = \ln G(w) - \ln G(0) 
    = \ln \frac{G(w)}{G(0)}\\
  \int_0^w \left(ib-\frac{w}{za}\right)dw' 
    &= \arrowvert ibw' - \frac{{w'}^2}{-4a}
    \arrowvert_0^w = ibw-\frac{w^2}{4a}\\
  G(0) = \int_{-\infty}^\infty g(x) dx &= \int_{-\infty}^\infty e^{-a(x-b)^2}
    = \sqrt{\frac{\pi}{a}}
\end{align}
From (2), (3), and (4), we get
\begin{align}
  G(w) = G(0) e^{ibw-\frac{w^2}{4a}} &= \sqrt{\frac{\pi}{a}} \quad e^{ibw} 
    e^{-\frac{w^2}{4a}}\\
  \text{or} \qquad
  \int_{-\infty}^\infty e^{-a(x-b)^2} e^{iqx}dx &= \sqrt{\frac{\pi}{a}}
    \: e^{ibq} e^{-\frac{q^2}{4a}}
\end{align}
\begin{align}
  g(x) &=F^{-1} \{G(w)\} = \frac{1}{2\pi} \int_{-\infty}^\infty 
    G(w)e^{-iwx}dw\\
  \text{and} \qquad \frac{dg(x)}{dx} &= \frac{1}{2\pi} \int_{-\infty}^\infty
    (-iw)G(w)e^{-iwx}dw\\
  &=F^{-1} \left\{-iwG(w)\right\}\\
  &\Rightarrow F\left\{\frac{dg(x)}{dx} \right\} = -(iwG(w))
\end{align}



\begin{equation}
  \pars{\frac{c}{d}}
  \braces{\frac{x}{y}}
  \bracks{\frac{a}{b}}
\end{equation}
\end{document}
